Use UTF-8 for special characters

Soundness.thy
@@ -5,50 +5,50 @@ begin
 lemma list_minus_set: "set (list_minus e xs) = set e - set xs"
   by (induction e) (auto)
 
-lemma free_in_context: "\<lbrakk> x \<in> set (fve_e e) ; \<Gamma> \<turnstile> e : \<tau> \<rbrakk> \<Longrightarrow> \<exists>\<tau>'. (x, \<tau>') \<in> \<Gamma>"
-proof (induction e arbitrary: \<Gamma> \<tau> x)
+lemma free_in_context: "⟦ x ∈ set (fve_e e) ; Γ ⊢ e : τ ⟧ ⟹ ∃τ'. (x, τ') ∈ Γ"
+proof (induction e arbitrary: Γ τ x)
   case (Var y)
   then show ?case using T.cases by fastforce
 next
-  case (Lam y \<tau>' e)
-  then have "x \<noteq> y" by (simp add: list_minus_set)
-  then have x: "x \<in> set (fve_e e)" using list_minus_set T.cases Lam by fastforce
-  from Lam(3) obtain \<tau>2 where "(y, \<tau>')#\<Gamma> \<turnstile> e : \<tau>2 \<and> \<tau> = (\<tau>' \<rightarrow> \<tau>2)" using T.cases by blast
-  then show ?case using Lam(1)[OF x] by (meson \<open>x \<noteq> y\<close> isin.simps(2)) 
+  case (Lam y τ' e)
+  then have "x ≠ y" by (simp add: list_minus_set)
+  then have x: "x ∈ set (fve_e e)" using list_minus_set T.cases Lam by fastforce
+  from Lam(3) obtain τ2 where "(y, τ')#Γ ⊢ e : τ2 ∧ τ = (τ' → τ2)" using T.cases by blast
+  then show ?case using Lam(1)[OF x] by (meson ‹x ≠ y› isin.simps(2))
 next
   case (App e1 e2)
-  from App(4) obtain \<tau>1 \<tau>2 where e: "\<Gamma> \<turnstile> e1 : \<tau>1 \<rightarrow> \<tau>2 \<and> \<Gamma> \<turnstile> e2 : \<tau>1" using T.cases by blast
-  from App have "x \<in> set (fve_e e1) \<or> x \<in> set (fve_e e2)" by simp
+  from App(4) obtain τ1 τ2 where e: "Γ ⊢ e1 : τ1 → τ2 ∧ Γ ⊢ e2 : τ1" using T.cases by blast
+  from App have "x ∈ set (fve_e e1) ∨ x ∈ set (fve_e e2)" by simp
   then show ?case using e App by blast
 next
   case Unit
   then show ?case by simp
 next
   case (Let y e1 e2)
-  then have x: "x \<in> set (fve_e e1) \<or> x \<in> set (fve_e e2)" using list_minus_set by fastforce
-  from Let(4) obtain \<tau>1 where "\<Gamma> \<turnstile> e1 : \<tau>1 \<and> (y, \<tau>1)#\<Gamma> \<turnstile> e2 : \<tau>" using T.cases by blast
+  then have x: "x ∈ set (fve_e e1) ∨ x ∈ set (fve_e e2)" using list_minus_set by fastforce
+  from Let(4) obtain τ1 where "Γ ⊢ e1 : τ1 ∧ (y, τ1)#Γ ⊢ e2 : τ" using T.cases by blast
   then show ?case using x Let
     by (metis Diff_iff Un_iff fve_e.simps(5) isin.simps(2) list.set_intros(1) list_minus_set set_append)
 qed
 
-lemma fun_ty_lam: "\<lbrakk> is_v_of_e e ; \<Gamma> \<turnstile> e : \<tau>1 \<rightarrow> \<tau>2 \<rbrakk> \<Longrightarrow> \<exists>x e'. e = (\<lambda>x:\<tau>1. e')"
+lemma fun_ty_lam: "⟦ is_v_of_e e ; Γ ⊢ e : τ1 → τ2 ⟧ ⟹ ∃x e'. e = (λx:τ1. e')"
   apply (cases e)
       apply auto
   using T.cases apply blast+
   done
 
-theorem progress: "[] \<turnstile> e : \<tau> \<Longrightarrow> is_v_of_e e \<or> (\<exists>e'. Step e e')"
-proof (induction "[] :: \<Gamma>" e \<tau> rule: T.induct)
+theorem progress: "[] ⊢ e : τ ⟹ is_v_of_e e ∨ (∃e'. Step e e')"
+proof (induction "[] :: Γ" e τ rule: T.induct)
   case T_UnitI
   then show ?case by simp
 next
-  case (T_VarI x \<tau>)
+  case (T_VarI x τ)
   then show ?case by simp
 next
-  case (T_AbsI x \<tau>1 e \<tau>2)
+  case (T_AbsI x τ1 e τ2)
   then show ?case by simp
 next
-  case (T_AppI e1 \<tau>1 \<tau>2 e2)
+  case (T_AppI e1 τ1 τ2 e2)
   note IH1 = T_AppI(2)
   note IH2 = T_AppI(4)
 
@@ -58,66 +58,66 @@ next
     from IH2 show ?thesis
     proof (elim disjE)
       assume "is_v_of_e e2"
-      from \<open>is_v_of_e e1\<close> T_AppI(1) have "\<exists>x e. e1 = (\<lambda>x:\<tau>1. e)" by (simp add: fun_ty_lam)
-      then have "\<exists>e'. Step (App e1 e2) e'" using \<open>is_v_of_e e2\<close> ST_BetaI by blast
+      from ‹is_v_of_e e1› T_AppI(1) have "∃x e. e1 = (λx:τ1. e)" by (simp add: fun_ty_lam)
+      then have "∃e'. Step (App e1 e2) e'" using ‹is_v_of_e e2› ST_BetaI by blast
       then show ?thesis by simp
     next
-      assume "\<exists>e2'. Step e2 e2'"
-      then show ?thesis using ST_App2I \<open>is_v_of_e e1\<close> by blast
+      assume "∃e2'. Step e2 e2'"
+      then show ?thesis using ST_App2I ‹is_v_of_e e1› by blast
     qed
   next
-    assume "\<exists>e1'. Step e1 e1'"
+    assume "∃e1'. Step e1 e1'"
     then obtain e1' where "Step e1 e1'" by blast
     then have "Step (App e1 e2) (App e1' e2)" by (rule ST_AppI)
     then show ?thesis by blast
   qed
 next
-  case (T_LetI e1 \<tau>1 x e2 \<tau>2)
+  case (T_LetI e1 τ1 x e2 τ2)
   then show ?case using ST_SubstI ST_LetI by blast
 qed
 
-definition closed :: "e \<Rightarrow> bool" where
-  "closed x \<equiv> fve_e x = []"
+definition closed :: "e ⇒ bool" where
+  "closed x ≡ fve_e x = []"
 
 
-corollary typeable_closed: "[] \<turnstile> e : \<tau> \<Longrightarrow> closed e"
+corollary typeable_closed: "[] ⊢ e : τ ⟹ closed e"
   unfolding closed_def
   using free_in_context last_in_set by fastforce
 
-lemma context_invariance: "\<lbrakk> \<Gamma> \<turnstile> e : \<tau> ; \<forall>x \<tau>'. x \<in> set (fve_e e) \<and> (x, \<tau>') \<in> \<Gamma> \<longrightarrow> (x, \<tau>')\<in>\<Gamma>' \<rbrakk> \<Longrightarrow> \<Gamma>' \<turnstile> e : \<tau>"
-proof (induction \<Gamma> e \<tau> arbitrary: \<Gamma>' rule: T.induct)
-  case (T_UnitI \<Gamma>)
+lemma context_invariance: "⟦ Γ ⊢ e : τ ; ∀x τ'. x ∈ set (fve_e e) ∧ (x, τ') ∈ Γ ⟶ (x, τ')∈Γ' ⟧ ⟹ Γ' ⊢ e : τ"
+proof (induction Γ e τ arbitrary: Γ' rule: T.induct)
+  case (T_UnitI Γ)
   then show ?case by (simp add: T.T_UnitI)
 next
-  case (T_VarI x \<tau> \<Gamma>)
+  case (T_VarI x τ Γ)
   then show ?case by (auto simp: T.T_VarI)
 next
-  case (T_AbsI y \<tau>1 \<Gamma> e \<tau>2)
+  case (T_AbsI y τ1 Γ e τ2)
   then show ?case by (simp add: T.T_AbsI list_minus_set)
 next
-  case (T_AppI \<Gamma> e1 \<tau>1 \<tau>2 e2)
+  case (T_AppI Γ e1 τ1 τ2 e2)
   then show ?case by auto (metis (mono_tags, lifting) T.T_AppI)
 next
-  case (T_LetI e1 \<tau>1 x e2 \<tau>2)
+  case (T_LetI e1 τ1 x e2 τ2)
   then show ?case apply auto
     by (smt DiffI T.T_LetI empty_iff insertE isin.simps(2) list.set(1) list.set(2) list_minus_set) 
 qed
 
-lemma substitution: "\<lbrakk> (x, \<tau>')#\<Gamma> \<turnstile> e : \<tau> ; [] \<turnstile> v : \<tau>' \<rbrakk> \<Longrightarrow> \<Gamma> \<turnstile> esubst_e v x e : \<tau>"
-proof (induction e arbitrary: \<Gamma> \<tau> v x \<tau>')
+lemma substitution: "⟦ (x, τ')#Γ ⊢ e : τ ; [] ⊢ v : τ' ⟧ ⟹ Γ ⊢ esubst_e v x e : τ"
+proof (induction e arbitrary: Γ τ v x τ')
   case (Var y)
   then show ?case
   proof (cases "x = y")
     case True
-    then have "\<tau> = \<tau>'" using Var T.cases by fastforce
+    then have "τ = τ'" using Var T.cases by fastforce
     then show ?thesis using True Var context_invariance by fastforce
   next
     case False
     then show ?thesis using Var context_invariance by simp
   qed
 next
-  case (Lam y \<sigma> e)
-  let ?lam = "\<lambda> y : \<sigma> . e"
+  case (Lam y σ e)
+  let ?lam = "λ y : σ . e"
   from Lam show ?case
   proof (cases "x = y")
     case True
@@ -126,51 +126,51 @@ next
       by (smt Diff_iff Lam.prems(1) True context_invariance fve_e.simps(2) insert_iff isin.simps(2) list.simps(15) list_minus_set)
   next
     case False
-    then obtain \<tau>2 where P: "\<tau> = (\<sigma> \<rightarrow> \<tau>2)" using Lam(2) T.cases by blast
-    then have "(y, \<sigma>)#(x, \<tau>')#\<Gamma> \<turnstile> e : \<tau>2" using T.cases Lam by blast
-    then have "(x, \<tau>')#(y, \<sigma>)#\<Gamma> \<turnstile> e : \<tau>2" using context_invariance False by force
+    then obtain τ2 where P: "τ = (σ → τ2)" using Lam(2) T.cases by blast
+    then have "(y, σ)#(x, τ')#Γ ⊢ e : τ2" using T.cases Lam by blast
+    then have "(x, τ')#(y, σ)#Γ ⊢ e : τ2" using context_invariance False by force
     then show ?thesis using False Lam T_AbsI P by simp
   qed
 next
   case (App e1 e2)
-  from \<open>(x, \<tau>') # \<Gamma> \<turnstile> App e1 e2 : \<tau>\<close> obtain \<tau>1 where P: "((x, \<tau>') # \<Gamma> \<turnstile> e1 : \<tau>1 \<rightarrow> \<tau>) \<and> ((x, \<tau>') # \<Gamma> \<turnstile> e2 : \<tau>1)" using T.cases by blast
+  from ‹(x, τ') # Γ ⊢ App e1 e2 : τ› obtain τ1 where P: "((x, τ') # Γ ⊢ e1 : τ1 → τ) ∧ ((x, τ') # Γ ⊢ e2 : τ1)" using T.cases by blast
   then show ?case using T_AppI App by fastforce
 next
   case Unit
   then show ?case apply auto using T_UnitI T.cases by blast
 next
   case (Let y e1 e2)
-  from Let(3) obtain \<tau>1 where P: "(x, \<tau>')#\<Gamma> \<turnstile> e1 : \<tau>1 \<and> (y, \<tau>1)#(x, \<tau>')#\<Gamma> \<turnstile> e2 : \<tau>" using T.cases by blast
+  from Let(3) obtain τ1 where P: "(x, τ')#Γ ⊢ e1 : τ1 ∧ (y, τ1)#(x, τ')#Γ ⊢ e2 : τ" using T.cases by blast
   from Let show ?case
   proof (cases "x = y")
     case True
     then have x: "esubst_e v x (Let y e1 e2) = Let y (esubst_e v x e1) e2" by simp
-    then have e1: "\<Gamma> \<turnstile> esubst_e v x e1 : \<tau>1" using Let P by blast
-    from True Let have e2: "(y, \<tau>1) # \<Gamma> \<turnstile> e2 : \<tau>" by (smt P context_invariance isin.simps(2))
+    then have e1: "Γ ⊢ esubst_e v x e1 : τ1" using Let P by blast
+    from True Let have e2: "(y, τ1) # Γ ⊢ e2 : τ" by (smt P context_invariance isin.simps(2))
     then show ?thesis using T_LetI[OF e1 e2] x by simp
   next
     case False
-    then have "(x, \<tau>')#(y, \<tau>1)#\<Gamma> \<turnstile> e2 : \<tau>" using P context_invariance by fastforce
+    then have "(x, τ')#(y, τ1)#Γ ⊢ e2 : τ" using P context_invariance by fastforce
     then show ?thesis
       by (smt False Let.IH(1) Let.IH(2) Let.prems(2) P T_LetI empty_iff esubst_e.simps(5) list.set(1) set_ConsD)
   qed
 qed
 
-theorem preservation: "\<lbrakk> [] \<turnstile> e : \<tau> ; Step e e' \<rbrakk> \<Longrightarrow> [] \<turnstile> e' : \<tau>"
-proof (induction "[] :: \<Gamma>" e \<tau> arbitrary: e' rule: T.induct)
+theorem preservation: "⟦ [] ⊢ e : τ ; Step e e' ⟧ ⟹ [] ⊢ e' : τ"
+proof (induction "[] :: Γ" e τ arbitrary: e' rule: T.induct)
 case T_UnitI
   then show ?case using Step.cases by blast
 next
-  case (T_VarI x \<tau>)
+  case (T_VarI x τ)
   then show ?case using Step.cases by blast
 next
-  case (T_AbsI x \<tau>1 e \<tau>2)
+  case (T_AbsI x τ1 e τ2)
   then show ?case using Step.cases by blast
 next
-  case (T_AppI e1 \<tau>1 \<tau>2 e2)
-  from \<open>App e1 e2 \<longrightarrow> e'\<close> show ?case
+  case (T_AppI e1 τ1 τ2 e2)
+  from ‹App e1 e2 ⟶ e'› show ?case
   proof cases
-    case (ST_BetaI x \<tau> e)
+    case (ST_BetaI x τ e)
     then show ?thesis using substitution T.cases T_AppI by blast
   next
     case (ST_AppI e2)
@@ -180,8 +180,8 @@ next
     then show ?thesis using T_AppI T.T_AppI by blast
   qed
 next
-  case (T_LetI e1 \<tau>1 x e2 \<tau>2)
-  from \<open>Let x e1 e2 \<longrightarrow> e'\<close> show ?case
+  case (T_LetI e1 τ1 x e2 τ2)
+  from ‹Let x e1 e2 ⟶ e'› show ?case
   proof (cases)
     case ST_SubstI
     then show ?thesis using substitution T.cases T_LetI by blast
@@ -191,18 +191,18 @@ next
   qed
 qed
 
-definition stuck :: "e \<Rightarrow> bool" where
-  "stuck e \<equiv> \<not>(is_v_of_e e \<or> (\<exists>e'. Step e e'))"
+definition stuck :: "e ⇒ bool" where
+  "stuck e ≡ ¬(is_v_of_e e ∨ (∃e'. Step e e'))"
 
-inductive Steps :: "e \<Rightarrow> e \<Rightarrow> bool" (infix "\<longrightarrow>*" 70) where
+inductive Steps :: "e ⇒ e ⇒ bool" (infix "⟶*" 70) where
   refl: "Steps e e"
-| trans: "\<lbrakk> Steps e1 e2 ; Step e2 e3 \<rbrakk> \<Longrightarrow> Steps e1 e3"
+| trans: "⟦ Steps e1 e2 ; Step e2 e3 ⟧ ⟹ Steps e1 e3"
 
-lemma multi_preservation: "\<lbrakk> e \<longrightarrow>* e' ; [] \<turnstile> e : \<tau> \<rbrakk> \<Longrightarrow> [] \<turnstile> e' : \<tau>"
+lemma multi_preservation: "⟦ e ⟶* e' ; [] ⊢ e : τ ⟧ ⟹ [] ⊢ e' : τ"
   apply (induction e e' rule: Steps.induct)
   using preservation by blast+
 
-corollary soundness: "\<lbrakk> [] \<turnstile> e : \<tau> ; e \<longrightarrow>* e' \<rbrakk> \<Longrightarrow> \<not>(stuck e')"
+corollary soundness: "⟦ [] ⊢ e : τ ; e ⟶* e' ⟧ ⟹ ¬(stuck e')"
   unfolding stuck_def
   using progress multi_preservation by blast
 
